Update the definition of types

Semantic/CC/Syntax/CaptureSet.lean
@@ -20,4 +20,36 @@ instance CaptureSet.instEmptyCollection :
 instance CaptureSet.instUnion : Union (CaptureSet s) where
   union := CaptureSet.union
 
+def Var.rename : Var k s1 -> Rename s1 s2 -> Var k s2
+| .bound x, f => .bound (f.var x)
+| .free n, _ => .free n
+
+def CaptureSet.rename : CaptureSet s1 -> Rename s1 s2 -> CaptureSet s2
+| .empty, _ => .empty
+| .union cs1 cs2, ρ => .union (cs1.rename ρ) (cs2.rename ρ)
+| .var x, ρ => .var (x.rename ρ)
+| .cvar x, ρ => .cvar (x.rename ρ)
+
+theorem CaptureSet.rename_id {cs : CaptureSet s} :
+    cs.rename (Rename.id) = cs := by
+  induction cs
+  case empty => rfl
+  case union ih1 ih2 => simp [CaptureSet.rename, ih1, ih2]
+  case var x => cases x <;> rfl
+  case cvar x => cases x <;> rfl
+
+theorem CaptureSet.rename_comp {cs : CaptureSet s1} {f : Rename s1 s2} {g : Rename s2 s3} :
+    (cs.rename f).rename g = cs.rename (f.comp g) := by
+  induction cs generalizing s2 s3
+  case empty => rfl
+  case union ih1 ih2 => simp [CaptureSet.rename, ih1, ih2]
+  case var x =>
+    cases x
+    · simp [CaptureSet.rename, Var.rename]; rfl
+    · simp [CaptureSet.rename, Var.rename]
+  case cvar x =>
+    cases x
+    · simp [CaptureSet.rename, Var.rename]; rfl
+    · simp [CaptureSet.rename, Var.rename]
+
 end CC
