Semantic/CC/Syntax/Ty.lean
@@ -16,16 +16,25 @@ inductive TySort : Type where
 | exi : TySort
 
 inductive Ty : TySort -> Sig -> Type where
+-- shape types
 | top : Ty .shape s
 | tvar : BVar s .tvar -> Ty .shape s
-| arrow : Ty .shape s -> Ty .shape (s,x) -> Ty .shape s
+| arrow : Ty .capt s -> Ty .exi (s,x) -> Ty .shape s
 | poly : Ty .shape s -> Ty .shape (s,X) -> Ty .shape s
+-- capturing types
+| capt : CaptureSet s -> Ty .shape s -> Ty .capt s
+-- existential types
+| exi : Ty .capt (s,C) -> Ty .exi s
+| typ : Ty .capt s -> Ty .exi s
 
 def Ty.rename : Ty sort s1 -> Rename s1 s2 -> Ty sort s2
 | .top, _ => .top
 | .tvar x, f => .tvar (f.var x)
 | .arrow T1 T2, f => .arrow (T1.rename f) (T2.rename (f.lift))
 | .poly T1 T2, f => .poly (T1.rename f) (T2.rename (f.lift))
+| .capt cs T, f => .capt (cs.rename f) (T.rename f)
+| .exi T, f => .exi (T.rename (f.lift))
+| .typ T, f => .typ (T.rename f)
 
 def Ty.rename_id {T : Ty sort s} : T.rename (Rename.id) = T := by
   induction T
@@ -33,6 +42,10 @@ def Ty.rename_id {T : Ty sort s} : T.rename (Rename.id) = T := by
   case tvar => rfl
   case arrow ih1 ih2 => simp [Ty.rename, Rename.lift_id, ih1, ih2]
   case poly ih1 ih2 => simp [Ty.rename, Rename.lift_id, ih1, ih2]
+  case capt ih2 =>
+    simp [Ty.rename, ih2, CaptureSet.rename_id]
+  case exi ih => simp [Ty.rename, Rename.lift_id, ih]
+  case typ ih => simp [Ty.rename, ih]
 
 theorem Ty.rename_comp {T : Ty sort s1} {f : Rename s1 s2} {g : Rename s2 s3} :
     (T.rename f).rename g = T.rename (f.comp g) := by
@@ -41,6 +54,9 @@ theorem Ty.rename_comp {T : Ty sort s1} {f : Rename s1 s2} {g : Rename s2 s3} :
   case tvar => rfl
   case arrow ih1 ih2 => simp [Ty.rename, Rename.lift_comp, ih1, ih2]
   case poly ih1 ih2 => simp [Ty.rename, Rename.lift_comp, ih1, ih2]
+  case capt ih => simp [Ty.rename, CaptureSet.rename_comp, ih]
+  case exi ih => simp [Ty.rename, Rename.lift_comp, ih]
+  case typ ih => simp [Ty.rename, ih]
 
 theorem Ty.weaken_rename_comm {T : Ty sort s1} {f : Rename s1 s2} :
     (T.rename Rename.succ).rename (f.lift (k:=k0)) = (T.rename f).rename (Rename.succ) := by
